backend/RTL.v
@@ -282,7 +282,7 @@ Inductive step: state -> trace -> state -> Prop :=
                   m')
   | exec_function_external:
       forall s ef args res t m m',
-      external_call ef (Genv.find_symbol ge) args m t res m' ->
+      external_call ef ge args m t res m' ->
       step (Callstate s (External ef) args m)
          t (Returnstate s res m')
   | exec_return:
