backend/Reloadproof.v
@@ -813,6 +813,10 @@ Lemma symbols_preserved:
   Genv.find_symbol tge id = Genv.find_symbol ge id.
 Proof (@Genv.find_symbol_transf _ _ _ transf_fundef prog).
 
+Lemma varinfo_preserved:
+  forall b, Genv.find_var_info tge b = Genv.find_var_info ge b.
+Proof (@Genv.find_var_info_transf _ _ _ transf_fundef prog).
+
 Lemma sig_preserved:
   forall f, funsig (transf_fundef f) = LTLin.funsig f.
 Proof.
@@ -1310,7 +1314,8 @@ Proof.
   intros [res' [tm' [A [B [C D]]]]]. 
   left; econstructor; split.
   apply plus_one. eapply exec_function_external; eauto. 
-  eapply external_call_symbols_preserved; eauto. exact symbols_preserved.
+  eapply external_call_symbols_preserved; eauto.
+  exact symbols_preserved. exact varinfo_preserved.
   econstructor; eauto.
   simpl. rewrite Locmap.gss. auto.
   intros. rewrite Locmap.gso. auto. 
