backend/Tailcallproof.v
@@ -240,6 +240,10 @@ Lemma symbols_preserved:
   forall (s: ident), Genv.find_symbol tge s = Genv.find_symbol ge s.
 Proof (Genv.find_symbol_transf transf_fundef prog).
 
+Lemma varinfo_preserved:
+  forall b, Genv.find_var_info tge b = Genv.find_var_info ge b.
+Proof (Genv.find_var_info_transf transf_fundef prog).
+
 Lemma functions_translated:
   forall (v: val) (f: RTL.fundef),
   Genv.find_funct ge v = Some f ->
@@ -557,7 +561,8 @@ Proof.
   intros [res' [m2' [A [B [C D]]]]].
   left. exists (Returnstate s' res' m2'); split.
   simpl. econstructor; eauto.
-  eapply external_call_symbols_preserved; eauto. exact symbols_preserved.
+  eapply external_call_symbols_preserved; eauto.
+  exact symbols_preserved. exact varinfo_preserved.
   constructor; auto. 
 
 (* returnstate *)
