backend/Tunnelingproof.v
@@ -160,6 +160,10 @@ Lemma symbols_preserved:
   Genv.find_symbol tge id = Genv.find_symbol ge id.
 Proof (@Genv.find_symbol_transf _ _ _ tunnel_fundef p).
 
+Lemma varinfo_preserved:
+  forall b, Genv.find_var_info tge b = Genv.find_var_info ge b.
+Proof (@Genv.find_var_info_transf _ _ _ tunnel_fundef p).
+
 Lemma sig_preserved:
   forall f, funsig (tunnel_fundef f) = funsig f.
 Proof.
@@ -335,7 +339,8 @@ Proof.
   (* external function *)
   simpl. left; econstructor; split.
   eapply exec_function_external; eauto.
-  eapply external_call_symbols_preserved; eauto. exact symbols_preserved.
+  eapply external_call_symbols_preserved; eauto.
+  exact symbols_preserved. exact varinfo_preserved.
   simpl. econstructor; eauto. 
   (* return *)
   inv H3. inv H1.
